Convert to type system from verasco

Classes/Galois.v
@@ -1,13 +1,6 @@
 Require Export Base.
-Require Import Classes.Joinable.
-Require Import Instances.Preorder.
-Require Import PreorderedSet.
 
-Class Galois (A A' : Type) `{A'_preorder: PreorderedSet A'} : Type :=
-{
-  γ : A' -> ℘ A;
-  gamma_monotone : monotone γ;
-}.
+Class Galois (A A' : Type) : Type :=  γ : A -> ℘ A'.
 Arguments γ : simpl never.
 Hint Extern 10 (γ _ _) => constructor : soundness.
 
@@ -16,33 +9,101 @@ Ltac gamma_destruct := repeat
   | x : γ _  _ |- _ => inv x
   end.
 
-Lemma gamma_preorder {A A'} `{A_galois : Galois A A'}: forall (a' a2' : A') (a : A), 
-    preorder a' a2' -> γ a' a -> γ a2' a.
-Proof.
-  intros a a' b Hpre Hgamma.
-  pose proof gamma_monotone as Hmono.
-  unfold monotone in Hmono. apply Hmono in Hpre.
-  destruct Hpre. auto with soundness.
-Qed.
+Definition gamma_bot {A A'} `{Galois A A'} : (A+⊥) → A' → Prop :=
+  λ a : A+⊥, match a with
+             | Bot => λ _, False
+             | NotBot x => λ y, γ x y
+             end.
 
-Lemma gamma_join_left {A A'} `{A'_joinable : Joinable A'} 
-  `{A_galois : @Galois A A' T_preorder} : ∀ (a : A) (a'1 a'2 : A'),
-  γ a'1 a → γ (join_op a'1 a'2) a.
-Proof. 
-  intros. apply (gamma_preorder a'1). 
-  apply join_upper_bound_left. assumption.
-Qed.
+Instance galois_bot {A A'} `{Galois A A'} : Galois (A+⊥) A' := gamma_bot.
 
-Lemma gamma_join_right {A A'} `{A'_joinable : Joinable A'} 
-  `{A_galois : @Galois A A' T_preorder} : ∀ (a : A) (a'1 a'2 : A'),
-  γ a'2 a → γ (join_op a'1 a'2) a.
-Proof. 
-  intros. apply (gamma_preorder a'2). 
-  apply join_upper_bound_right. assumption.
-Qed.
+Definition gamma_top {A A'} `{Galois A A'} : (A+⊤) → ℘ A' :=
+  λ a : A+⊤, match a with
+             | Top => λ _, True
+             | NotTop x => λ y, γ x y
+             end.
+Instance galois_top {A A'} `{Galois A A'} : Galois (A+⊤) A' := gamma_top.
 
-Ltac apply_widen :=
-  match goal with
-  | H : preorder ?a ?b, I : γ ?a ?c |- γ ?b ?c =>
-      eapply gamma_preorder; apply H + apply I
-  end.
+Section galois_functions.
+  Context {A A' B B' : Type}  
+          `{A_galois : Galois A A', B_galois : Galois B B'}.
+
+  Inductive gamma_fun : (A → B) → (A' → B') → Prop :=
+    | gamma_fun_cons : ∀ (f : A → B) (g : A' → B'), 
+        (∀ (a : A) (a' : A'),
+        γ a a' → γ (f a) (g a')) → gamma_fun f g.
+
+  Global Instance galois_fun : Galois (A → B) (A' → B') := gamma_fun.
+End galois_functions.
+Hint Constructors gamma_fun : soundness.
+
+Section galois_unit.
+  Definition gamma_unit (u v : unit) : Prop := True.
+
+  Global Instance galois_unit : Galois unit unit := gamma_unit.
+End galois_unit.
+Hint Unfold gamma_unit : soundness.
+
+Section galois_pairs.
+  Context {A A' B B'} `{A_galois : Galois A A'} `{B_galois : Galois B B'}.
+
+  Inductive gamma_pairs : prod A B → prod A' B' → Prop :=
+    | gamma_pairs_cons : ∀ p q,
+        γ (fst p) (fst q) → γ (snd p) (snd q) → gamma_pairs p q.
+
+  Global Instance galois_pairs : Galois (A*B)%type (A'*B')%type := gamma_pairs.
+End galois_pairs.
+Hint Constructors gamma_pairs : soundness.
+
+Section galois_sums.
+  Context {A A' B B'} `{GA : Galois A A'} `{GB : Galois B B'}.
+
+  Definition gamma_sum : (A+B) → ℘ (A'+B') := λ s, λ s',
+      match s, s' with 
+      | inl x, inl y => γ x y
+      | inr x, inr y => γ x y
+      | _, _ => False
+      end.
+
+  Global Instance galois_sum : Galois (A+B) (A'+B') := gamma_sum.
+End galois_sums.
+
+Section galois_identity.
+  Context {A A'} `{A_galois : Galois A A'}.
+
+  Definition gamma_identity (ia' : Identity A) 
+                            (ia : Identity A') : Prop :=
+    match ia', ia with
+    | identity a', identity a => γ a' a
+    end.
+
+  Global Instance galois_identity : Galois (Identity A) (Identity A') :=
+    gamma_identity.
+End galois_identity.
+
+Section galois_option.
+  Context {A A'} `{A_galois : Galois A A'}.
+
+  Inductive gamma_optionA : optionA A → option A' → Prop :=
+    | gamma_noneA : gamma_optionA NoneA None
+    | gamma_SomeornoneA_none : ∀ a, 
+        gamma_optionA (SomeOrNoneA a) None
+    | gamma_SomeA_Some : ∀ a' a, γ a' a → gamma_optionA (SomeA a') (Some a)
+    | gamma_Someornone_Some : ∀ a' a, 
+        γ a' a →
+        gamma_optionA (SomeOrNoneA a') (Some a).
+  Hint Constructors gamma_optionA : soundness.
+
+  Inductive gamma_option : option A → option A' → Prop :=
+    | gamma_none : ∀ m, gamma_option None m
+    | gamma_Some_Some : ∀ a' a, γ a' a → gamma_option (Some a') (Some a).
+  Hint Constructors gamma_option : soundness.
+
+  Global Instance galois_optionA : Galois (optionA A) (option A') :=
+    gamma_optionA.
+
+  Global Instance galois_option : Galois (option A) (option A') :=
+    gamma_option.
+End galois_option.
+Hint Constructors gamma_optionA gamma_option : soundness.
+
