Classes/IsBool.v
@@ -1,5 +1,89 @@
-Class IsBool (M : Type -> Type)
-  (valType boolType : Type) : Type :=
+Require Export Base.
+Require Import Classes.Joinable Classes.Galois.
+
+Class and_op (A B : Type) : Type := and : A → A → B.
+Infix "&&" := and.
+
+Class and_op_sound (A A' : Type) {B B' : Type} `{Galois A A', Galois B B'}
+  `{and_op A B} `{and_op A' B'} : Prop :=
+  and_sound : ∀ (a1 a2 : A) (a1' a2' : A'),
+  γ a1 a1' →
+  γ a2 a2' →
+  γ (a1 && a2) (a1' && a2').
+
+Instance and_bool : and_op bool bool := andb.
+
+Instance and_top {A B : Type} `{and_op A B} : and_op (A+⊤) (B+⊤) :=
+  λ a1, λ a2, match a1, a2 with
+              | NotTop x, NotTop y => NotTop (x && y)
+              | _,_ => Top
+              end.
+
+Instance and_bot {A B : Type} `{and_op A B} : and_op (A+⊥) (B+⊥) :=
+  λ a1, λ a2, match a1, a2 with
+              | NotBot x, NotBot y => NotBot (x && y)
+              | _, _ => Bot
+              end.
+
+Class or_op  (A B : Type) : Type := or : A → A → B.
+Infix "||" := or.
+Class or_op_sound (A A' : Type) {B B' : Type} `{Galois A A', Galois B B'}
+  `{or_op A B} `{or_op A' B'} : Prop :=
+  or_sound : ∀ (a1 a2 : A) (a1' a2' : A'),
+  γ a1 a1' →
+  γ a2 a2' →
+  γ (a1 || a2) (a1' || a2').
+
+Instance or_bool : or_op bool bool := orb.
+
+Instance or_top {A B : Type} `{or_op A B} : or_op (A+⊤) (B+⊤) :=
+  λ a1, λ a2, match a1, a2 with
+              | NotTop x, NotTop y => NotTop (x || y)
+              | _, _ => Top
+              end.
+
+Instance or_bot {A B : Type} `{or_op A B} : or_op (A+⊥) (B+⊥) :=
+  λ a1, λ a2, match a1, a2 with
+              | NotBot x, NotBot y => NotBot (x || y)
+              | _, _ => Bot
+              end.
+
+Class neg_op (A B : Type) : Type := neg : A → B.
+Class neg_op_sound (A A' : Type) {B B' : Type} `{Galois A A', Galois B B'}
+  `{neg_op A B} `{neg_op A' B'} : Prop :=
+  neg_sound : ∀ (a : A) (a' : A'),
+  γ a a' →
+  γ (neg a) (neg a').
+
+Instance neg_bool : neg_op bool bool := negb.
+
+Instance neg_top {A B : Type} `{neg_op A B} : neg_op (A+⊤) (B+⊤) :=
+  λ a, match a with | NotTop x => NotTop (neg x) | Top => Top end.
+
+Instance neg_bot {A B : Type} `{neg_op A B} : neg_op (A+⊥) (B+⊥) :=
+  λ a, match a with | NotBot x => NotBot (neg x) | Bot => Bot end.
+
+Class if_op  (A B : Type) : Type := when : A → B → B → B.
+Class if_op_sound (A A' : Type) {B B' : Type} `{Galois A A', Galois B B'}
+  `{if_op A B} `{if_op A' B'} : Prop :=
+  if_sound : ∀ (g : A) (g' : A') (p1 p2 : B) (p1' p2' : B'),
+    γ g g' →
+    γ p1 p1' → 
+    γ p2 p2' →
+    γ (when g p1 p2) (when g' p1' p2').
+
+Instance if_bool {B : Type} : if_op bool B := 
+  λ (b : bool),
+  λ (p1 : B), λ (p2 : B),
+  if b then p1 else p2.
+
+Instance if_top {A B : Type} `{if_op A B} `{Joinable B B} : if_op (A+⊤) B :=
+  λ a, λ b1, λ b2, match a with
+                   | Top => b1 ⊔ b2
+                   | NotTop b => when b b1 b2
+                   end.
+
+(*Class IsBool (M : Type -> Type) (valType boolType : Type) : Type :=
 {
   ensure_bool  : valType -> M boolType;
   build_bool   : boolType -> M valType;
@@ -7,4 +91,4 @@ Class IsBool (M : Type -> Type)
   and_op       : boolType -> boolType -> M boolType;
   neg_op       : boolType -> M boolType;
   if_op        : boolType -> M unit -> M unit -> M unit;
-}.
+}.*)
