Classes/IsNat.v
@@ -1,4 +1,86 @@
-Class IsNat (M : Type -> Type)
+Require Export Base.
+Require Import Classes.Galois.
+
+Class plus_op (A B : Type) := plus : A → A → B.
+Infix "+" := plus.
+Class plus_op_sound (A A' : Type) {B B'} `{Galois A A', Galois B B'} 
+  `{plus_op A B} `{plus_op A' B'} : Prop :=
+  plus_sound : ∀ (a1 a2 : A) (a1' a2' : A'),
+  γ a1 a1' →
+  γ a2 a2' →
+  γ (a1 + a2) (a1' + a2').
+
+Instance nat_plus_op : plus_op nat nat := Nat.add.
+
+Instance top_plus_op_r {A B : Type} `{plus_op A B} : plus_op A (B+⊤) :=
+  λ a1 : A, λ a2 : A, NotTop (a1 + a2).
+
+Instance top_plus_op_l {A B : Type} `{plus_op A (B+⊤)} : plus_op (A+⊤) (B+⊤) :=
+  λ a1, λ a2, match a1, a2 with
+              | Top, _ | _, Top => Top
+              | NotTop x, NotTop y => x + y
+              end.
+
+Class mult_op (A B : Type) := mult : A → A → B.
+Infix "*" := mult.
+Class mult_op_sound (A A' : Type) {B B'} `{Galois A A', Galois B B'}
+  `{mult_op A B} `{mult_op A' B'} : Prop :=
+  mult_sound : ∀ (a1 a2 : A) (a1' a2' : A'),
+  γ a1 a1' →
+  γ a2 a2' →
+  γ (a1 * a2) (a1' * a2').
+
+Instance nat_mult_op : mult_op nat nat := Nat.mul.
+
+Instance top_mult_op_r {A B : Type} `{mult_op A B} : mult_op A (B+⊤) :=
+  λ a1 : A, λ a2 : A, NotTop (a1 * a2).
+
+Instance top_mult_op_l {A B : Type} `{mult_op A (B+⊤)} : mult_op (A+⊤) (B+⊤) :=
+  λ a1, λ a2, match a1, a2 with
+              | Top, _ | _, Top => Top
+              | NotTop x, NotTop y => x * y
+              end.
+
+Class eq_op (A B : Type) := eq : A → A → B.
+Infix "=" := eq.
+Class eq_op_sound (A A' : Type) {B B'} `{Galois A A', Galois B B'}
+  `{eq_op A B} `{eq_op A' B'} : Prop :=
+  eq_sound : ∀ (a1 a2 : A) (a1' a2' : A'),
+  γ a1 a1' →
+  γ a2 a2' →
+  γ (a1 = a2) (a1' = a2').
+
+Instance nat_eq_op : eq_op nat bool := Nat.eqb.
+
+Instance top_eq_op_r {A B : Type} `{eq_op A B} : eq_op A (B+⊤) :=
+  λ a1 : A, λ a2 : A, NotTop (a1 = a2).
+
+Instance top_eq_op_l {A B : Type} `{eq_op A (B+⊤)} : eq_op (A+⊤) (B+⊤) :=
+  λ a1, λ a2, match a1, a2 with
+              | Top, _ | _, Top => Top
+              | NotTop x, NotTop y => x = y
+              end.
+
+Class leb_op (A B : Type) := leb : A → A → B.
+Class leb_op_sound (A A' : Type) {B B'} `{Galois A A', Galois B B'}
+  `{leb_op A B} `{leb_op A' B'} : Prop :=
+  leb_sound : ∀ (a1 a2 : A) (a1' a2' : A'),
+  γ a1 a1' →
+  γ a2 a2' → 
+  γ (leb a1 a2) (leb a1' a2').
+
+Instance nat_leb_op : leb_op nat bool := Nat.leb.
+
+Instance top_leb_op_r {A B : Type} `{leb_op A B} : leb_op A (B+⊤) :=
+  λ a1, λ a2, NotTop (leb a1 a2).
+
+Instance top_leb_op_l {A B : Type} `{leb_op A (B+⊤)} : leb_op (A+⊤) (B+⊤) :=
+  λ a1, λ a2, match a1, a2 with
+              | Top, _ | _, Top => Top
+              | NotTop x, NotTop y => leb x y
+              end.
+
+(*Class IsNat (M : Type -> Type)
   (valType boolType natType : Type) : Type :=
 {
   ensure_nat  : valType -> M natType;
@@ -9,3 +91,4 @@ Class IsNat (M : Type -> Type)
   eq_op       : natType -> natType -> M boolType;
   le_op       : natType -> natType -> M boolType;
 }.
+*)
