Classes/Joinable.v
@@ -1,24 +1,155 @@
 Require Export Base.
-Require Import Classes.PreorderedSet.
+Require Import Classes.Galois.
 
-Class Joinable (T : Type) `{T_preorder : PreorderedSet T} : Type :=
+Class Joinable (A B : Type) : Type :=
 {
-  join_op : T -> T -> T;
-  join_idem : ∀ x, join_op x x = x;
-  join_upper_bound_left: forall t t', preorder t (join_op t t');
-  join_assoc : ∀ x y z : T, 
-    join_op x (join_op y z) = join_op (join_op x y) z;
+  join_op : A -> A -> B;
   join_comm : ∀ x y, join_op x y = join_op y x;
 }.
-
-Corollary join_upper_bound_right {T : Type} `{Joinable T} : ∀ t t',
-  preorder t' (join_op t t').
-Proof.
-  intros. rewrite join_comm. apply join_upper_bound_left.
-Qed.
-
 Arguments join_op : simpl never.
-Hint Resolve join_upper_bound_left join_upper_bound_right : soundness.
-Hint Rewrite @join_idem : soundness.
-
 Infix "⊔" := join_op (at level 40).
+
+Class JoinableSound (A B C : Type) 
+  `{Joinable A B} `{Galois A C} `{Galois B C} : Prop :=
+  join_sound : ∀ x y : A, γ x ∪ γ y ⊆ γ (x ⊔ y).
+
+Section joinable_functions.
+  Context {A B : Type} `{Joinable B B}.
+
+  Definition fun_join (f g : A → B) : A → B :=
+    λ a : A, (f a) ⊔ (g a).
+
+  Lemma fun_join_comm : ∀ f g,
+    fun_join f g = fun_join g f.
+  Proof.
+    intros f g. unfold fun_join. extensionality a.
+    rewrite join_comm. reflexivity.
+  Qed.
+
+  Global Instance functions_joinable : Joinable (A → B) (A → B) :=
+  {
+    join_comm := fun_join_comm;
+  }.
+End joinable_functions.
+
+Section joinable_top_l.
+  Context (A : Type) `{Joinable A (A+⊤)}.
+
+  Definition top_join (a a' : A+⊤) : A+⊤ :=
+    match a, a' with
+    | NotTop x, NotTop y => x ⊔ y
+    | _, _ => Top
+    end.
+
+  Global Instance top_joinable_l : Joinable (A+⊤) (A+⊤).
+  Proof.
+    split with (top_join). intros x y.
+    destruct x, y; simpl. 4: rewrite join_comm. 
+    all: reflexivity.
+  Defined.
+End joinable_top_l.
+
+Section joinable_top_r.
+  Context (A : Type) `{AJ : Joinable A A}.
+
+  Definition top_join_r (a a' : A) : A+⊤ := NotTop (a ⊔ a').
+
+  Global Instance top_joinable_r : Joinable A (A+⊤).
+  Proof.
+    split with top_join_r. intros. unfold top_join_r. rewrite join_comm.
+    reflexivity.
+  Defined.
+End joinable_top_r.
+
+Definition unit_join : unit -> unit -> unit :=
+    fun _ _ => tt.
+Hint Unfold unit_join : soundness.
+
+Global Instance unit_joinable : Joinable unit unit.
+Proof.
+  split with unit_join. destruct x, y; reflexivity.
+Defined.
+
+Section identity_joinable.
+  Context {A B : Type} `{Joinable A B}.
+
+  Definition identity_join (i j : Identity A) : Identity B :=
+    match i, j with
+    | identity a, identity a' => identity (a ⊔ a')
+    end.
+
+  Global Instance identity_joinable : Joinable (Identity A) (Identity B).
+  Proof.
+    split with identity_join. destruct x, y; simpl. rewrite join_comm.
+    reflexivity.
+  Defined.
+End identity_joinable.
+
+Section option_joinable.
+  Context {A : Type} `{A_joinable : Joinable A A}.
+
+  Definition option_join (m n : option A) : option A :=
+    match m, n with
+    | Some x, Some y => Some (x ⊔ y)
+    | _, _ => None
+    end.
+
+  Global Instance option_joinable : Joinable (option A) (option A).
+  Proof.
+    split with option_join. destruct x, y; simpl. rewrite join_comm.
+    all: reflexivity.
+  Defined.
+End option_joinable.
+
+Section optionA_joinable.
+  Context {A : Type} `{A_joinable : Joinable A A}.
+
+  Definition optionA_join
+    (st1 st2 : optionA A) : optionA A :=
+    match st1, st2 with
+    | NoneA, NoneA => NoneA
+    | SomeA x, SomeA y => SomeA (x ⊔ y)
+    | SomeA x, NoneA | NoneA, SomeA x =>  SomeOrNoneA x
+    | NoneA, SomeOrNoneA x | SomeOrNoneA x, NoneA => SomeOrNoneA x
+    | SomeA x, SomeOrNoneA y | SomeOrNoneA x, SomeA y => 
+        SomeOrNoneA (x ⊔ y)
+    | SomeOrNoneA x, SomeOrNoneA y => SomeOrNoneA (x ⊔ y)
+    end.
+  Hint Unfold optionA_join : soundness.
+
+  Global Instance optionA_joinable : Joinable (optionA A) (optionA A).
+  Proof.
+    split with optionA_join. destruct x, y; simpl; try rewrite join_comm;
+    reflexivity.
+  Defined.
+End optionA_joinable.
+
+Section joinable_pairs.
+  Context {A B A' B'} `{A_joinable : Joinable A A', B_joinable : Joinable B B'}.
+
+  Definition pair_join (p q : (A*B)%type) : (A'*B')%type :=
+    ((fst p) ⊔ (fst q), (snd p) ⊔ (snd q)).
+
+  Global Instance joinable_pairs : Joinable (A*B) (A'*B').
+  Proof.
+    split with pair_join. destruct x, y; simpl. unfold pair_join; simpl.
+    rewrite (join_comm a0 a), (join_comm b0 b). reflexivity.
+  Defined.
+End joinable_pairs.
+
+Section joinable_sums.
+    Context {A A' B B'} `{JA : Joinable A A', JB : Joinable B B'}.
+
+    Definition sum_join : (A+B) → (A+B) → (A'+B')+⊤ := 
+      λ s1, λ s2, match s1, s2 with
+                  | inl x, inl y => NotTop (inl (x ⊔ y))
+                  | inr x, inr y => NotTop (inr (x ⊔ y))
+                  | _, _ => Top
+                  end.
+
+    Global Instance joinable_sums : Joinable (A+B) ((A'+B')+⊤).
+    Proof.
+      split with sum_join. intros x y. unfold sum_join. destruct x, y; try
+      rewrite join_comm; reflexivity.
+    Defined.
+End joinable_sums.
