Classes/PreorderedSet.v
@@ -1,24 +1,149 @@
 Require Export Base.
+Require Import Classes.Galois Psatz.
 
-Class PreorderedSet (X : Type) : Type :=
+Create HintDb preorders.
+
+Class PreorderedSet (A : Type) : Type :=
 {
-  preorder : X -> X -> Prop;
-  preorder_refl: forall x, preorder x x;
-  preorder_trans: forall x y z, preorder x y -> preorder y z -> preorder x z;
+  preorder : A -> A -> Prop;
+  preorder_refl: ∀ x, preorder x x;
+  preorder_trans: ∀ x y z, preorder x y -> preorder y z -> preorder x z;
 }.
-Hint Resolve preorder_refl preorder_trans : soundness.
-Hint Extern 10 (preorder _ _) => constructor : soundness.
+Infix "⊑" := preorder (at level 40).
+Hint Resolve preorder_refl preorder_trans : preorders.
 
-Definition monotone {A B} `{A_pre : PreorderedSet A, B_pre : PreorderedSet B} :
-  (A -> B) -> Prop :=
-  fun f => forall (a a': A), preorder a a' -> preorder (f a) (f a').
-  
-Hint Unfold monotone : soundness.
+Class PreorderSound (A B : Type) `{PreorderedSet A} `{Galois A B} : Prop :=
+  preorder_sound : ∀ x y : A, x ⊑ y → γ x ⊆ γ y.
 
 Ltac pre_trans :=
   match goal with
-  | H : preorder ?a ?b, K : preorder ?b ?c  |- preorder ?a ?c =>
+  | H : ?a ⊑ ?b, K : ?b ⊑ ?c  |- ?a ⊑ ?c =>
       eapply preorder_trans; [apply H|assumption]
   end.
 
-Infix "⊑" := preorder (at level 40).
+Ltac proof_preorder R := 
+  split with (preorder:=R); autounfold with preorders;
+  [> intros x; (destruct x; eauto with preorders) + 
+               (constructor;intros; apply preorder_refl + assumption)| 
+     intros x y z Hxy Hyz; (destruct x, y, z + constructor;intros);
+     eauto with preorders; inversion Hxy; inversion Hyz; eauto with preorders ].
+
+Inductive bot_le {A} `{PreorderedSet A} : (A+⊥) → (A+⊥) → Prop :=
+  | bot_le_l : ∀ y, bot_le Bot y
+  | bot_le_not : ∀ x y, x ⊑ y → bot_le (NotBot x) (NotBot y).
+Hint Constructors bot_le : preorders.
+
+Instance preorder_bot {A} `{PreorderedSet A} : PreorderedSet (A+⊥).
+Proof.
+  proof_preorder bot_le.
+Defined.
+
+Inductive top_le {A} `{PreorderedSet A} : (A+⊤) → (A+⊤) → Prop :=
+  | top_le_r : ∀ x, top_le x Top 
+  | top_le_not : ∀ x y, x ⊑ y → top_le (NotTop x) (NotTop y).
+Hint Constructors top_le : preorders.
+
+Instance preorder_top {A} `{PreorderedSet A} : PreorderedSet (A+⊤).
+Proof. proof_preorder top_le. Defined.
+
+Section preordered_functions.
+  Context {A A' : Type} `{A_preorder : PreorderedSet A'}.
+
+  Inductive pointwise_ordering : (A → A') → (A → A') → Prop :=
+  | pointwise_cons : ∀ f g,  
+      (∀ x, preorder (f x) (g x)) → pointwise_ordering f g.
+  Hint Constructors pointwise_ordering : preorders.
+
+  Global Instance preordered_function_spaces : PreorderedSet (A->A').
+  Proof. proof_preorder pointwise_ordering. Defined.
+End preordered_functions.
+Hint Constructors pointwise_ordering : soundness.
+
+Section preordered_pairs.
+  Context {A B : Type} 
+    `{A_preorder : PreorderedSet A, B_preorder : PreorderedSet B}.
+
+  Inductive preorder_pair_le : prod A B → prod A B → Prop :=
+    | preorder_pair_cons : ∀ a b c d,
+        preorder a c → preorder b d → preorder_pair_le (a,b) (c,d).
+  Hint Constructors preorder_pair_le : preorders.
+
+  Global Instance preorder_pairs : PreorderedSet (A * B)%type.
+  Proof.
+    proof_preorder preorder_pair_le. 
+  Defined.
+
+  Lemma preorder_pair_spec : ∀ p q, ∃ a b c d,
+    preorder p q <-> preorder (a, b) (c, d).
+  Proof.
+    intros. destruct p, q. exists a, b, a0, b0. reflexivity.
+  Qed.
+End preordered_pairs.
+Hint Constructors preorder_pair_le : soundness.
+
+Definition unit_le (u v : unit) : Prop := True.
+Hint Unfold unit_le : preorders.
+
+Instance preorder_unit : PreorderedSet unit.
+Proof. proof_preorder unit_le. Defined.
+
+Section preordered_sets_le.
+  Context {A : Type}.
+
+  Inductive preordered_set_le : (℘ A) → (℘ A) → Prop :=
+    | preordered_set_le_cons : ∀ (s t : A → Prop),
+        (∀ x, s x → t x) → preordered_set_le s t.
+  Hint Constructors preordered_set_le : preorders.
+
+  Global Instance types_to_prop : PreorderedSet (℘ A).
+  Proof. proof_preorder preordered_set_le. Defined.
+
+End preordered_sets_le.
+Hint Constructors preordered_set_le : soundness.
+
+Section identity_preorder.
+  Context {A} `{A_preorder : PreorderedSet A}.
+
+  Definition identity_le (i1 i2 : Identity A) : Prop :=
+    match i1, i2 with
+    | identity a1, identity a2 => preorder a1 a2
+    end.
+  Hint Unfold identity_le : preorders.
+
+  Global Instance identity_preorder : PreorderedSet (Identity A).
+  Proof. proof_preorder identity_le. Defined.
+End identity_preorder.
+
+Section option_preorder.
+  Context {A} `{A_preorder : PreorderedSet A}.
+
+  Inductive option_le : option A → option A → Prop :=
+    | option_le_none : ∀ m, option_le m None
+    | option_le_just : ∀ x y, preorder x y → option_le (Some x) (Some y).
+  Hint Constructors option_le : preorders.
+
+  Global Instance option_preorder : PreorderedSet (option A).
+  Proof. proof_preorder option_le. Defined.
+End option_preorder.
+Hint Constructors option_le : soundness.
+
+Global Instance preorder_nat : PreorderedSet nat.
+Proof. proof_preorder le; eauto with arith. Defined.
+
+Section optionA_preorder.
+  Context {A : Type} `{A_preorder : PreorderedSet A}.
+
+  Inductive optionA_le : optionA A → optionA A → Prop :=
+    | optionA_le_none : optionA_le NoneA NoneA
+    | optionA_le_none_justornone : ∀ y, optionA_le NoneA (SomeOrNoneA y)
+    | optionA_le_just : ∀ x y, preorder x y → optionA_le (SomeA x) (SomeA y)
+    | optionA_le_justornone_r : ∀ x y, preorder x y →
+        optionA_le (SomeA x) (SomeOrNoneA y)
+    | optionA_le_justornone : ∀ x y, preorder x y →
+        optionA_le (SomeOrNoneA x) (SomeOrNoneA y).
+  Hint Constructors optionA_le : preorders.
+
+  Global Instance optionA_preorder : PreorderedSet (optionA A).
+  Proof. proof_preorder optionA_le. Defined.
+End optionA_preorder.
+Hint Constructors optionA_le : soundness.
