SharedInterpreter.v
@@ -6,83 +6,100 @@ Require Import Classes.IsBool.
 Require Import Classes.Monad.MonadState.
 Require Import Classes.Monad.MonadFail.
 Require Import Classes.Monad.MonadExcept.
+Require Import Types.Stores.
 
-Definition extract_build_val {M : Type -> Type} {valType boolType natType : Type}
-    `{M_monad : Monad M, nat_inst : IsNat M valType boolType natType, 
-               bool_inst : IsBool M valType boolType}
-    (v : cvalue) : M valType :=
-  match v with
-  | VNat n => n' <- extract_nat n; build_nat n'
-  | VBool b => b' <- extract_bool b; build_bool b'
+Definition foo := (nat + bool)%type.
+
+Definition ensure_type (subType : Type)
+  {M : Type → Type} `{MF : MonadFail M}
+  {valType : Type}
+  `{SubType subType valType}
+  (n : valType) : M subType :=
+  match project n with
+  | Some x =>  returnM (M:=M) x
+  | None => fail
   end.
 
 Fixpoint shared_eval_expr 
-    {M : Type -> Type} {valType boolType natType : Type}
-    `{M_monad : Monad M, 
-      store_inst : MonadState (total_map valType) M,
-      nat_inst  : IsNat M valType boolType natType, 
-      bool_inst : IsBool M valType boolType}
+    {valType boolType natType : Type} {M : Type → Type} `{MM : !Monad M}
+    `{MF : !MonadFail M} `{MS : !MonadState (store valType) M}
+    `{SB : SubType boolType valType}
+    `{SN : SubType natType valType}
+    `{PO : plus_op natType natType}
+    `{MO : mult_op natType natType}
+    `{EO : eq_op natType boolType}
+    `{LO : leb_op natType boolType}
+    `{NO : neg_op boolType boolType}
+    `{AO : and_op boolType boolType}
     (e : expr) : M valType :=
   match e with
-  | EVal v =>
-      extract_build_val v
+  | EVal v => fail
   | EVar x =>
       s <- get;
-      returnM (s x)
+      returnM (M:=M) (s x)
   | EPlus e1 e2 => 
       v1 <- shared_eval_expr e1 ;
       v2 <- shared_eval_expr e2 ;
-      n1 <- ensure_nat v1 ;
-      n2 <- ensure_nat v2 ;
-      n <- plus_op n1 n2 ;
-      build_nat n
+      n1 <- ensure_type natType v1 ;
+      n2 <- ensure_type natType v2 ;
+      n <- returnM (M:=M) (n1 + n2) ;
+      returnM (M:=M) (inject n)
   | EMult e1 e2 => 
       v1 <- shared_eval_expr e1 ;
       v2 <- shared_eval_expr e2 ;
-      n1 <- ensure_nat v1 ;
-      n2 <- ensure_nat v2 ;
-      n <- mult_op n1 n2 ;
-      build_nat n
+      n1 <- ensure_type natType v1 ;
+      n2 <- ensure_type natType v2 ;
+      n <- returnM (M:=M) (n1 * n2) ;
+      returnM (inject n)
   | EEq e1 e2 =>
       v1 <- shared_eval_expr e1 ;
       v2 <- shared_eval_expr e2 ;
-      n1 <- ensure_nat v1 ;
-      n2 <- ensure_nat v2 ;
-      b <- eq_op n1 n2 ;
-      build_bool b
+      n1 <- ensure_type natType v1 ;
+      n2 <- ensure_type natType v2 ;
+      b <- returnM (M:=M) (n1 = n2) ;
+      returnM (M:=M) (inject b)
   | ELe e1 e2 =>
       v1 <- shared_eval_expr e1 ;
       v2 <- shared_eval_expr e2 ;
-      n1 <- ensure_nat v1 ;
-      n2 <- ensure_nat v2 ;
-      b <- le_op n1 n2;
-      build_bool b
+      n1 <- ensure_type natType v1 ;
+      n2 <- ensure_type natType v2 ;
+      b <- returnM (M:=M) (leb n1 n2);
+      returnM (M:=M) (inject b)
   | ENot e1 =>
       v1 <- shared_eval_expr e1 ;
-      b1 <- ensure_bool v1 ;
-      b <- neg_op b1;
-      build_bool b
+      b1 <- ensure_type boolType v1 ;
+      b <- returnM (M:=M) (neg b1);
+      returnM (M:=M) (inject b)
   | EAnd e1 e2 =>
       v1 <- shared_eval_expr e1 ;
       v2 <- shared_eval_expr e2 ;
-      b1 <- ensure_bool v1 ;
-      b2 <- ensure_bool v2 ;
-      b <- and_op b1 b2 ;
-      build_bool b
+      b1 <- ensure_type boolType v1 ;
+      b2 <- ensure_type boolType v2 ;
+      b <- returnM (M:=M) (b1 && b2) ;
+      returnM (M:=M) (inject b)
   end.
 
 Open Scope com_scope.
 
 Fixpoint shared_ceval 
-  {M : Type -> Type} {valType natType boolType : Type}
-  `{M_fail : MonadFail M, 
-    store : MonadState (total_map valType)  M, 
-    M_except : ∀ A, MonadExcept M A, 
-    nat_inst : IsNat M valType boolType natType, 
-    bool_inst : IsBool M valType boolType}
-  (c : com) : M unit :=
+    {valType boolType natType : Type} 
+    {M : Type → Type} 
+    `{MM : !Monad M}
+    `{MF : !MonadFail M} 
+    `{MS : !MonadState (store valType) M}
+    `{ME : !MonadExcept M unit} (c : com) 
+    `{SubType boolType valType}
+    `{SubType natType valType}
+    `{PO : plus_op natType natType}
+    `{MO : mult_op natType natType}
+    `{EO : eq_op natType boolType}
+    `{LO : leb_op natType boolType}
+    `{NO : neg_op boolType boolType}
+    `{AO : and_op boolType boolType}
+    `{IO : if_op boolType (M unit)}
+    : M unit :=
   match c with
-  | CSkip => returnM tt
+  | CSkip => returnM (M:=M) tt
   | c1 ;c; c2 =>
       (shared_ceval c1) ;; (shared_ceval c2)
   | x ::= a => 
@@ -91,8 +108,8 @@ Fixpoint shared_ceval
       put (t_update s x v)
   | CIf b c1 c2 => 
       v <- shared_eval_expr b ;
-      b' <- ensure_bool v ;
-      if_op b' (shared_ceval c1) (shared_ceval c2)
+      b' <- ensure_type boolType v ;
+      when b' (shared_ceval c1) (shared_ceval c2)
   | TRY c1 CATCH c2 => 
       catch (shared_ceval c1) (shared_ceval c2)
   | CFail => fail
