Soundness.v
@@ -1,8 +1,6 @@
 Require Export Base.
 Require Export Instances.Galois.
 Require Import Classes.Galois.
-Require Import Classes.IsBool.
-Require Import Classes.IsNat.
 Require Import Classes.Joinable.
 Require Import Classes.Monad.
 Require Import Classes.Monad.MonadFail.
@@ -12,11 +10,6 @@ Require Import Coq.Arith.Arith.
 Require Import Coq.Arith.Even.
 Require Import Coq.Arith.PeanoNat.
 Require Import Instances.Except.
-Require Import Instances.IsBool.AbstractBoolean.
-Require Import Instances.IsBool.Boolean.
-Require Import Instances.IsNat.Interval.
-Require Import Instances.IsNat.Nat.
-Require Import Instances.IsNat.Parity.
 Require Import Instances.Joinable.
 Require Import Instances.Monad.
 Require Import Instances.Preorder.
@@ -30,12 +23,9 @@ Require Import Types.Maps.
 Require Import Types.Parity.
 Require Import Types.State.
 Require Import Types.Stores.
+Require Import Classes.IsBool.
 
 Hint Extern 0 (γ _ _) => progress gamma_destruct : soundness.
-
-Axiom gamma_pure_none : ∀ {M M' : Type → Type} `{Monad M, Monad M'} {A A' :
-  Type}  `{Galois (M A) (M' (option A'))} (c : M A), γ (returnM (M:=M') None) c.
-Hint Resolve gamma_pure_none : soundness.
 
 (* Soundness of unit *)
 Lemma gamma_unit_sound :
@@ -46,71 +36,56 @@ Hint Resolve gamma_unit_sound : soundness.
 (* Soundness of functions *)
 Lemma gamma_fun_apply {A A' B B'} `{Galois A A', Galois B B'}
     (f : A -> B) (f' : A' -> B') x x' :
-  γ f' f -> γ x' x -> γ (f' x') (f x).
+  γ f f' -> γ x x' -> γ (f x) (f' x').
 Proof. 
   eauto with soundness.
 Qed.
 Hint Extern 3 (γ (?f ?x) (?g ?y)) => apply gamma_fun_apply : soundness.
 
-Lemma gamma_fun_applied {A A' B B'} `{Galois A A', Galois B B'}
-    (f : A -> B) (f' : A' -> B') :
-      (forall x x', γ x' x -> γ (f' x') (f x)) ->
-        γ f' f.
-Proof. 
-  eauto with soundness.
-Qed.
-(*Hint Resolve gamma_fun_applied : soundness.*)
-
 (* Soundness of monadic operations *)
-Lemma some_sound : ∀ (A A' : Type) `{A_galois : Galois A A'},
-  γ (Some (A:=A')) (Some (A:=A)).
+Lemma some_sound {A A' : Type} `{Galois A A'} : ∀ a a', 
+  γ a a' →
+  γ (Some a) (Some a').
 Proof.
   eauto with soundness.
 Qed.
 
-Lemma bind_option_sound : ∀ (A A' B B' : Type) `{Galois A A', Galois B B'},
-  γ (bindM (M:=option) (A:=A') (B:=B')) 
-        bindM.
+Lemma bind_option_sound {A A' B B'} `{Galois A A', Galois B B'} : 
+  ∀ m m' f f', 
+  γ m m' → γ f f' →
+  γ (bind_option m f) (bind_option m' f').
 Proof.
   unfold bindM; simpl.
   repeat constructor. intros.
-  destruct a', a; eauto with soundness.
+  destruct m, m'; eauto with soundness.
 Qed.
 Hint Resolve bind_option_sound : soundness.
 
-Instance option_sound : SoundMonad option option :=
-{
-  return_sound := some_sound;
-  bind_sound := bind_option_sound;
-}.
-
-Lemma someA_sound : ∀ A A' `{A_galois : Galois A A'},
-  γ (SomeA (A:=A')) Some.
+Lemma someA_sound {A A' : Type} `{GA : Galois A A'} : ∀ (a : A) (a' : A'),
+  γ a a' → 
+  γ (SomeA a) (Some a').
 Proof.
   eauto with soundness.
 Qed.
 
 Lemma bind_optionA_sound (A A' B B' : Type) `{Galois A A', Galois B B'} :
-  γ (bindM (M:=optionA) (A:=A') (B:=B')) bindM.
+  ∀ (m : optionA A) (m' : option A') 
+    (f : A → optionA B) (f' : A' → option B'),
+  γ m m' → γ f f' →
+  γ (bind_optionA m f) (bind_option m' f').
 Proof.
-  unfold bindM; simpl.
-  constructor; intros ma ma' Hma. constructor; intros mf mf' Hmf.
-  destruct ma, ma' as [a'| |a']; simpl; eauto with soundness.
-  inversion Hma as [Ha |? |? |?? Ha];subst.
-  inversion Hmf as [?? Hf]; subst.
-  apply Hf in Ha. all: destruct (mf' a'); eauto with soundness.
+  intros m m' f f' Hm Hf. destruct m, m'; eauto with soundness.
+  - inversion Hm; subst; clear Hm. gamma_destruct. apply H1 in H3.
+    cbv. destruct (f a), (f' a0); simpl; try constructor;  eauto with
+      soundness.
+  - inversion Hm; subst; clear Hm. gamma_destruct. cbv. destruct (f a);
+    constructor.
 Qed.
-
-Instance abstract_option_sound : SoundMonad option optionA :=
-{
-  return_sound := someA_sound;
-  bind_sound := bind_optionA_sound;
-}.
 
 Lemma bind_state_sound {S S'} `{Galois S S'} : ∀ (A A' B B' : Type)
   `{Galois A A', Galois B B'},
   γ
-    (bind_state (S:=S') (A:=A') (B:=B'))
+    (bind_state (S:=S) (A:=A) (B:=B))
     bind_state.
 Proof. 
   unfold bind_state. constructor; intros st st' Hst.
@@ -123,478 +98,117 @@ Qed.
 Hint Resolve bind_state_sound : soundness.
 
 Section stateT.
-  Context {M M' : Type → Type} `{SoundMonad M M'}.
-  Context {S S' : Type} `{Galois S S'} `{!Inhabited S, !Inhabited S'}.
+  Context {M M' : Type → Type} `{Monad M, Monad M'}.
+  Context {GM : ∀ A A', Galois A A' → Galois (M A) (M' A')}.
+  Context {S S' : Type} `{Galois S S'}.
+  Context {RS : return_sound M M'}.
+  Context {BS : bind_sound M M'}.
 
-  Lemma return_stateT_sound : ∀ A A' `{A_galois : Galois A A'},
-    γ (return_stateT (S:=S') (M:=M') (A:=A')) (return_stateT (A:=A)).
+  Lemma return_stateT_sound {A A'} `{Galois A A'} : 
+    γ (return_stateT (S:=S) (M:=M) (A:=A)) 
+      (return_stateT (S:=S') (M:=M') (A:=A')).
   Proof.
-    unfold return_stateT. eauto 10 using return_sound with soundness.
+    unfold return_stateT. constructor. intros a a' Ha. constructor.
+    intros s s' Hs. eauto with soundness.
   Qed.
 
-  Lemma bind_stateT_sound : ∀ (A A' B B' : Type) `{Galois A A', Galois B B'},
-    γ (bind_stateT (A:=A') (B:=B') (S:=S') (M:=M')) bind_stateT.
+  Lemma bind_stateT_sound {A A' B B'} `{Galois A A', Galois B B'} : 
+    ∀ (m : StateT S M A) (m' : StateT S' M' A')
+      (f : A → StateT S M B) (f' : A' → StateT S' M' B'),
+    γ m m' → γ f f' → 
+    γ (bind_stateT m f) (bind_stateT m' f').
   Proof.
-    intros. unfold bind_stateT. repeat constructor; intros. repeat eapply
-    gamma_fun_apply; eauto with soundness. constructor; intros p p' Hp.
-    destruct p, p'. repeat eapply gamma_fun_apply; eauto with soundness.
+    intros. unfold bind_stateT. repeat constructor; intros s s' Hs. 
+    apply bindM_sound.
+    apply gamma_fun_apply; assumption. constructor. intros p p' Hp.
+    destruct p, p'. eauto with soundness.
   Qed.
-
-  Global Instance stateT_sound : SoundMonad (StateT S M) (StateT S' M') :=
-  {
-    return_sound := return_stateT_sound;
-    bind_sound := bind_stateT_sound;
-  }.
 End stateT.
 
 Section optionT.
-  Context {M M' : Type → Type} `{SoundMonad M M'}.
+  Context {M M' : Type → Type}.
+  Context `{RS : return_sound M M'}.
+  Context {BS : bind_sound M M'}.
 
-  Lemma someT_sound : ∀ A A' `{Galois A A'},
-    γ (λ a, returnM (M:=M') (Some (A:=A') a)) (λ a, returnM (M:=M) (Some a)).
+  Lemma someT_sound {A A'} `{Galois A A'} : ∀ a a',
+    γ a a' →
+    γ (returnM (M:=M) (Some a)) (returnM (M:=M') (Some a')).
   Proof. 
-    intros. constructor. intros. eapply gamma_fun_apply; eauto with soundness. 
+    intros. eapply gamma_fun_apply; eauto with soundness. 
   Qed.
 
-  Lemma bind_optionT_sound : ∀ (A A' B B' : Type) `{Galois A A', Galois B B'},
-    γ (bind_optionT (A:=A') (B:=B') (M:=M')) bind_optionT.
+  Lemma bind_optionT_sound {A A' B B'} `{Galois A A', Galois B B'} : 
+    ∀ (m : optionT M A) (m' : optionT M' A')
+      (f : A → optionT M B) (f' : A' → optionT M' B'),
+    γ m m' → γ f f' → 
+    γ (bind_optionT m f) (bind_optionT m' f').
   Proof. 
-    intros. unfold bind_optionT, optionT. repeat constructor; intros. 
-    repeat eapply gamma_fun_apply; eauto with soundness.
-  Qed.
-
-  Global Instance optionT_sound : SoundMonad (optionT M) (optionT M') :=
-  {
-    return_sound := someT_sound;
-    bind_sound := bind_optionT_sound;
-  }.
+    intros. eapply BS. assumption. constructor; intros a a' Ha.
+    gamma_destruct; eauto with soundness. admit.
+  Admitted.
 End optionT.
 
 Section optionAT.
-  Context {M M' : Type → Type} `{SoundMonad M M'}.
+  Context {M M' : Type → Type}.
+  Context `{RS : return_sound M M'} {BS : bind_sound M M'}.
 
-  Lemma someAT_sound : ∀ A A' `{Galois A A'},
-    γ (λ a : A', returnM (M:=M') (SomeA a)) (λ a, returnM (M:=M) (Some a)).
+  Lemma someAT_sound {A A'} `{Galois A A'} : ∀ a a',
+    γ a a' →
+    γ (returnM (SomeA a)) (returnM (Some a')).
   Proof. eauto with soundness. Qed.
 
-  Lemma bind_optionAT_sound : ∀ (A A' B B' : Type) `{Galois A A', Galois B B'},
-    γ (bind_optionAT (A:=A') (B:=B') (M:=M')) bind_optionT.
+  Lemma bind_optionAT_sound {A A' B B'} `{Galois A A', Galois B B'} : 
+    ∀ (m : optionAT M A) (m' : optionT M' A') 
+      (f : A → optionAT M B) (f' : A' → optionT M' B'),
+    γ m m' → γ f f' →
+    γ (bind_optionAT m f) (bind_optionT m' f').
   Proof.
-    intros. constructor; intros Ma Ma' HMa.
-    constructor; intros f f' Hf'. unfold bind_optionAT, bind_optionT.
-    unfold optionT, optionAT.
-    repeat apply gamma_fun_apply; eauto with soundness. 
-    constructor; intros m m' Hm. 
-    destruct m; inversion Hm; subst; eauto with soundness.
-    - rewrite <- bind_id_right. eapply gamma_fun_apply.
-      eauto with soundness.
-      constructor; intros m m' Hm'. destruct m'; eauto with soundness.
-    - eauto with soundness. admit.
+    intros. unfold bind_optionAT, bind_optionT, optionAT, optionT.
+    apply bindM_sound; try assumption.
+    constructor; intros a a' Ha.
+    inversion Ha; subst; eauto with soundness.
+    - rewrite <- bind_id_right. admit.
+    - rewrite <- bind_id_right. apply bindM_sound; eauto with soundness.
+      constructor. intros. destruct a, a'; eauto with soundness.
   Admitted.
 
   Lemma lift_optionAT_sound {A A'} `{Galois A A'} :
-    γ (lift_optionAT (M:=M') (A:=A')) (lift_optionT (A:=A)).
+    γ (lift_optionAT (M:=M) (A:=A)) (lift_optionT (A:=A')).
   Proof.
     unfold lift_optionAT, lift_optionT, optionAT, optionT.
-    repeat constructor. intros.
-    repeat eapply gamma_fun_apply; eauto with soundness.
+    repeat constructor. intros. apply bindM_sound; eauto with soundness.
   Qed.
 
-  Global Instance optionAT_sound : SoundMonad (optionT M) (optionAT M') :=
-  {
-    return_sound := someAT_sound;
-    bind_sound := bind_optionAT_sound;
-  }.
 End optionAT.
-
-(* Soundness of parity operations *)
-
-Lemma gamma_par_extract_n_n : forall n,
-  γ (extract_par n) n.
-Proof.
-  intros. autounfold with soundness. 
-  destruct (Nat.even n) eqn:Hpar. 
-  - rewrite Nat.even_spec in Hpar. eauto with soundness.
-  - pose proof Nat.negb_even. 
-    constructor.
-    rewrite <- Nat.odd_spec. rewrite <- Nat.negb_even, Bool.negb_true_iff.
-    assumption.
-Qed.
-
-Lemma parity_plus_sound :
-  γ parity_plus plus.
-Proof.
-  autounfold with soundness. repeat constructor. intros.
-  destruct a', a'0; eauto with soundness.
-Qed.
-
-Lemma parity_mult_sound :
-  γ parity_mult mult.
-Proof. 
-  autounfold with soundness. repeat constructor; intros.
-  destruct a', a'0; gamma_destruct; try constructor; eauto with soundness.
-Qed.
-
-Hint Rewrite Nat.eqb_eq : soundness.
-Lemma parity_eq_sound :
-  γ parity_eq Nat.eqb. 
-Proof. 
-  repeat constructor. intros. destruct a', a'0; simpl; try constructor.
-  gamma_destruct. assert (a ≠ a0). unfold not. intro; subst.
-  apply (Nat.Even_Odd_False a0); auto. rewrite Nat.eqb_neq; auto.
-  gamma_destruct. assert (a ≠ a0). unfold not. intro; subst.
-  apply (Nat.Even_Odd_False a0); auto. rewrite Nat.eqb_neq; auto.
-Qed.
-
-Lemma extract_par_sound : forall n,
-  γ (extract_par n) n.
-Proof. 
-  intros. unfold extract_par. destruct (Nat.even n) eqn:Hpar; repeat constructor.
-  rewrite <- Nat.even_spec; auto.
-  rewrite <- Nat.odd_spec. unfold Nat.odd. rewrite Hpar. reflexivity.
-Qed.
-
-(* Monadic versions of parity operations *)
-Lemma ensure_par_sound {M M'} `{SoundMonad M M'} 
-  {M'_fail : MonadFail M'} {M_fail : MonadFail M} :
-  γ (ensure_par (M:=M')) ensure_nat.
-Proof.
-  constructor; intros a a' Hgamma. destruct a; inv Hgamma; subst; simpl; eauto
-  with soundness.
-Admitted.
-Hint Resolve ensure_par_sound : soundness.
-
-Lemma extract_parM_sound {M M'} `{SoundMonad M M'} : forall n,
-  γ (extract_parM n) (extract_natM n). 
-Proof. 
-  intros. unfold extract_parM, extract_natM. 
-  repeat eapply gamma_fun_apply; eauto using extract_par_sound with soundness. 
-Qed. 
-Hint Resolve extract_parM_sound : soundness.
-
-Lemma pplusM_sound {M M'} `{SoundMonad M M'} : 
-  γ pplusM plusM.
-Proof. 
-  unfold pplusM, plusM.
-  repeat constructor; eauto using parity_plus_sound with soundness. 
-Qed.
-Hint Resolve pplusM_sound : soundness.
-
-Lemma pmultM_sound {M M'} `{SoundMonad M M'} :
-  γ pmultM multM.
-Proof.
-  unfold pmultM, multM.
-  repeat constructor; eauto using parity_mult_sound with soundness. 
-Qed.
-Hint Resolve pmultM_sound : soundness.
-
-Lemma peqM_sound {M M'} `{SoundMonad M M'} :
-  γ peqM eqbM.
-Proof.
-  unfold peqM, eqbM.
-  repeat constructor; eauto using parity_eq_sound with soundness.
-Qed.
-Hint Resolve peqM_sound : soundness.
-
-Lemma pleM_sound {M M'} `{SoundMonad M M'} :
-  γ pleM lebM.
-Proof.
-  unfold pleM, lebM.
-  repeat constructor; eauto with soundness.
-Qed.
-Hint Resolve pleM_sound : soundness.
-
-Lemma build_parity_sound {M M'} `{SoundMonad M M'} :
-  γ build_parity build_natural.
-Proof.
-  unfold build_parity, build_natural.
-  repeat constructor; eauto with soundness.
-Qed.
-Hint Resolve build_parity_sound : soundness.
-
-(* Soundness of operations on intervals *)
-Lemma iplus_sound : γ iplus plus.
-Proof.
-  repeat constructor; gamma_destruct; simpl in *; lia.
-Qed.
-
-Lemma iplusM_sound {M M'} `{SoundMonad M M'} :
-  γ iplusM plusM.
-Proof. 
-  unfold iplusM, plusM.
-  repeat constructor; intros. eauto using iplus_sound with soundness.
-Qed.
-Hint Resolve iplusM_sound : soundness.
-
-Lemma imult_sound : γ imult mult.
-Proof.
-  repeat constructor. 
-  - rewrite interval_min_mult. gamma_destruct; simpl in *.
-    apply Coq.Arith.Mult.mult_le_compat; auto.
-  - rewrite interval_max_mult. gamma_destruct; simpl in *.
-    apply Coq.Arith.Mult.mult_le_compat; auto.
-Qed.
-
-Lemma imultM_sound {M M'} `{SoundMonad M M'} :
-  γ imultM multM.
-Proof.
-  unfold imultM, multM.
-  repeat constructor; intros. eauto using imult_sound with soundness.
-Qed.
-Hint Resolve imultM_sound : soundness.
-
-Lemma ileqb_sound : γ ileqb leb.
-Proof.
-  constructor; intros n i Hn; constructor; intros m j Hm.
-  unfold ileqb. gamma_destruct; simpl in *.
-  destruct (max i <? min j) eqn:Hij. 
-  rewrite Nat.ltb_lt in Hij.
-  assert (n <=? m = true) as Hnm. rewrite Nat.leb_le. lia. rewrite Hnm.
-  auto with soundness. destruct (max j <? min i) eqn:Hji.
-  rewrite Nat.ltb_lt in Hji. rewrite Nat.ltb_ge in Hij.
-  assert (n <=? m = false) as Hnm. apply leb_correct_conv. lia.
-  rewrite Hnm. constructor. reflexivity. constructor.
-Qed.
-
-Lemma ilebM_sound {M M'} `{SoundMonad M M'} :
-  γ ileM lebM.
-Proof.
-  unfold ileM, lebM.
-  repeat constructor; intros. eauto using ileqb_sound with soundness.
-Qed.
-Hint Resolve ileqb_sound : soundness.
-
-Lemma ieqb_sound : γ ieqb Nat.eqb.
-Proof. 
-  unfold ieqb. constructor; intros n i Hin; constructor; intros m j Hjm.
-  inversion Hin as [i' n' Hmini Hmaxi]; subst; clear Hin.
-  inversion Hjm as [j' m' Hminj Hmaxj]; subst; clear Hjm. simpl in *.
-  destruct (max i <? min j) eqn:Hij. assert (n =? m = false) as Hnm.
-  rewrite Nat.eqb_neq. rewrite Nat.ltb_lt in Hij. lia. rewrite Hnm.
-  auto with soundness. destruct (min i =? max i) eqn:Hii; eauto with soundness.
-  destruct (max i =? min j) eqn:Hieqj; eauto with soundness.
-  destruct (min j =? max j) eqn:Hjj; eauto with soundness. simpl.
-  rewrite Nat.eqb_eq in Hii, Hieqj, Hjj. rewrite Hii in Hmini.
-  assert (n = max i). apply Nat.le_antisymm; assumption. subst.
-  rewrite Hjj in Hminj. assert (m = max j). apply Nat.le_antisymm; assumption.
-  subst. rewrite Hjj in Hieqj. rewrite <- Nat.eqb_eq in Hieqj.
-  rewrite Hieqj. eauto with soundness.
-Qed.
-
-Lemma ieqM_sound {M M'} `{SoundMonad M M'} : γ ieqM eqbM.
-Proof.
-  unfold ieqM, eqbM. repeat constructor; eauto using ieqb_sound with soundness.
-Qed.
-Hint Resolve ieqM_sound : soundness.
-
-Lemma build_interval_sound {M M'} `{SoundMonad M M'} :
-  γ build_interval build_natural.
-Proof.
-  unfold build_interval, build_natural.
-  repeat constructor; simpl; gamma_destruct; eauto with soundness.
-Qed.
-Hint Resolve build_interval_sound : soundness.
-
-Lemma extract_interval_sound {M M'} `{SoundMonad M M'} : forall n,
-  γ (extract_interval n) (extract_natM n).
-Proof.
-  unfold extract_interval, extract_natM.
-  intros. apply gamma_fun_apply. eauto with soundness. repeat constructor.
-Qed.
-Hint Resolve extract_interval_sound : soundness.
-
-Lemma ensure_interval_sound {M M'} `{SoundMonad M M'} 
-  {M_fail : MonadFail M} {M'_fail : MonadFail M'} : 
-  γ ensure_interval ensure_nat.
-Proof.
-  constructor; intros v v' Hv. inversion Hv; subst.
-Admitted.
-Hint Resolve ensure_interval_sound : soundness.
-
-(* Soundness of operations on booleans *)
-
-Lemma ab_and_sound :
-  γ and_ab andb.
-Proof. 
-  repeat constructor; intros. 
-  destruct_all bool; destruct_all abstr_bool; eauto with soundness.
-Qed.
-
-Lemma ab_or_sound :
-  γ or_ab orb.
-Proof. 
-  repeat constructor; intros.
-  destruct_all bool; destruct_all abstr_bool; eauto with soundness.
-Qed.
-
-Lemma ab_neg_sound :
-  γ neg_ab negb.
-Proof. 
-  repeat constructor; intros. 
-  destruct_all bool; destruct_all abstr_bool; eauto with soundness.
-Qed.
-
-Lemma extract_bool_sound : forall x,
-  γ (VAbstrBool (extract_ab x)) (VBool x).
-Proof. 
-  intros. destruct x; eauto with soundness.
-Qed.
-
-(* Monadic operations on abstract booleans *)
-
-Lemma ensure_abool_sound {M M'} `{SoundMonad M M'} 
-  {M_fail : MonadFail M} {M'_fail : MonadFail M'} :
-  γ ensure_abool ensure_bool.
-Proof. 
-  constructor. intros a b Hab. unfold ensure_abool, ensure_bool.
-Admitted.
-Hint Resolve ensure_abool_sound : soundness.
-
-Lemma neg_abM_sound {M M'} `{SoundMonad M M'} :
-  γ neg_abM negbM.
-Proof.
-  unfold neg_abM, negbM. 
-  repeat constructor; eauto using ab_neg_sound with soundness.
-Qed.
-Hint Resolve neg_abM_sound : soundness.
-
-Lemma and_abM_sound {M M'} `{SoundMonad M M'} :
-  γ and_abM andbM.
-Proof.
-  unfold and_abM, andbM. 
-  repeat constructor; eauto using ab_and_sound with soundness.
-Qed.
-Hint Resolve and_abM_sound : soundness.
-
-Lemma extract_abM_sound {M M'} `{SoundMonad M M'} : forall b,
-  γ (extract_abM b) (extract_boolean b).
-Proof. 
-  unfold extract_abM, extract_boolean. destruct b; eauto with soundness.
-Qed.
-Hint Resolve extract_abM_sound : soundness.
-
-Lemma build_boolean_sound {M M'} `{SoundMonad M M'} :
-  γ build_abool build_boolean.
-Proof.
-  unfold build_abool, build_boolean.
-  repeat constructor; eauto with soundness.
-Qed.
-Hint Resolve build_boolean_sound : soundness.
-
-(* Soundness of operations on stores *)
-
-(*Lemma store_get_sound : forall s,
-  γ (abstract_store_get s) (store_get s).
-Proof.
-  repeat constructor. inv H0. apply H1. inv H0; assumption.
-  inv H; assumption.
-Qed.
-Hint Resolve store_get_sound : soundness.*)
-
-Lemma t_update_sound : forall (ast : abstract_store) (st : store) x p n,
-  γ ast st ->
-  γ p n ->
-  γ (t_update ast x p) (t_update st x n).
-Proof. 
-  unfold t_update. repeat constructor; eauto with soundness.
-  intros x'. destruct (beq_string x x'); eauto with soundness.
-Qed.
 
 (* Soundness of interpreters *)
 
-Definition ConcreteState := optionT (StateT store (optionT Identity)).
+Definition avalue := ((parity+⊤)+(abstr_bool+⊤))%type.
+Definition ConcreteState := optionT (StateT (store cvalue) (optionT Identity)).
 
-Definition AbstractState := 
-  optionAT (StateT abstract_store (optionT Identity)).
-
-Lemma extract_build_val_sound : forall (v : cvalue),
-  γ 
-    (extract_build_val (M:=AbstractState) 
-        (valType:=avalue)
-        (nat_inst:=isnat_parity AbstractState)
-        (bool_inst:=(abstract_boolean_type)) v) 
-    (extract_build_val (M:=ConcreteState) (valType:=cvalue) v).
-Proof.
-  destruct v; repeat constructor; eauto using extract_par_sound with soundness. 
-  destruct b; auto with soundness.
-Qed.
-Hint Resolve extract_build_val_sound : soundness.
+Definition AbstractState := optionAT (StateT (store (avalue+⊤)) (optionT Identity)).
 
 Theorem eval_expr_sound : forall a,
   γ 
-    (shared_eval_expr (M:=AbstractState) (nat_inst:=isnat_parity AbstractState) 
-      (bool_inst:=(abstract_boolean_type)) (valType:=avalue) a) 
-    (shared_eval_expr (M:=ConcreteState) (valType:=cvalue) a).
+    (shared_eval_expr (M:=AbstractState) (valType:=avalue+⊤)
+    (boolType:=abstr_bool+⊤) (natType:=parity+⊤) a) 
+    (shared_eval_expr (M:=ConcreteState) (valType:=cvalue) 
+    (boolType:=bool) (natType:=nat) a).
 Proof.
-  intros. induction a; repeat constructor; simpl; intros.
-  - auto using gamma_fun_apply with soundness.
-  - auto using gamma_fun_apply with soundness. gamma_destruct.
-    auto.
-  - intros. repeat apply gamma_fun_apply; eauto with soundness.
-  - repeat apply gamma_fun_apply. admit. auto. constructor; intros.
-    repeat apply gamma_fun_apply. admit. auto. constructor; intros.
-    repeat apply gamma_fun_apply. admit. admit. auto. admit. auto.
+  intros. induction a; repeat constructor; simpl; intros. 
+  - auto with soundness.
+  - auto with soundness. 
+  - auto with soundness.
+  - apply gamma_fun_apply. 2: assumption. admit.
+  - admit.
 Admitted.
 Hint Resolve eval_expr_sound : soundness.
 
-Section sound_if.
-  Context {M M' : Type → Type} `{SoundMonad M M'} `{MonadFail M'}.
-  Hypothesis M'_joinable : ∀ (T : Type) {T_pre : PreorderedSet T}, 
-    Joinable T → Joinable (M' T).
-
-Lemma sound_if_op : 
-  γ (eval_if_abstract (M:=M')) (eval_if (M:=M)).
-Proof.
-  constructor; intros b ab Hab. constructor; intros m m' Hm. 
-  constructor; intros m2 m2' Hm2. 
-  destruct b, ab; simpl; eauto with soundness. inversion Hab. discriminate.
-  apply gamma_join_left. apply Hm. inversion Hab. discriminate.
-  apply gamma_join_right. apply Hm2.
-Qed.
-End sound_if.
-
-(*Lemma sound_eval_catch :
-  γ (eval_catch_abstract) (eval_catch).
-Proof.
-  intros s1' s1 H s2' s2. intros H0 a b H1. 
-  unfold γ in H, H0; simpl in H, H0; unfold gamma_fun in H, H0.
-  unfold eval_catch_abstract, eval_catch.
-  pose proof H1; apply H in H1.
-  destruct (s1' a).
-  - destruct (s1 b). 
-    + apply H1.
-    + apply H1.
-    + inversion H1.
-  - reflexivity.
-  - destruct (s1 b).  
-    + inversion H1.
-    + inversion H1.
-    + apply H0. apply H1.
-  - destruct (s1 b).
-    + eapply widen. apply join_upper_bound_left.
-      apply H1.
-    + inversion H1.
-    + unfold γ in H1; simpl in H1.
-      eapply widen. apply join_upper_bound_right. unfold gamma; simpl.
-      pose proof H1. apply H0 in H1.  apply H1.
-Qed.
-Hint Resolve sound_eval_catch : soundness.
-*)
-  (*
-Lemma sound_fail : 
-  γ fail_abstract fail.
-Proof.
-  unfold fail_abstract, fail. intros ???. auto.
-Qed.
-Hint Resolve sound_fail : soundness.
-*)
-
-Theorem sound_interpreter:
-  forall c, γ (shared_ceval 
-                    (M:=AbstractState) 
-                    (nat_inst:=isnat_parity AbstractState)
-                    c) 
-                  (shared_ceval (M:=ConcreteState) c).
+Theorem sound_interpreter: ∀ c, 
+  γ (shared_ceval (M:=AbstractState) (valType:=avalue+⊤)
+    (boolType:=(abstr_bool+⊤)) (natType:=(parity+⊤)) c) 
+    (shared_ceval (M:=ConcreteState) (valType:=cvalue)
+    (boolType:=bool) (natType:=nat) c).
 Proof.
   induction c; simpl. 
   - eauto with soundness.
