Types/Parity.v
@@ -1,86 +1,102 @@
 Require Export Base.
-Require Import Coq.Arith.Arith.
-Require Import Coq.Arith.PeanoNat.
-Require Import Coq.Arith.Even.
-Require Import Coq.Sets.Partial_Order.
-Require Import Types.AbstractBool.
+Require Import Coq.Arith.Arith Coq.Arith.PeanoNat Coq.Arith.Even
+  Coq.Sets.Partial_Order Types.AbstractBool Classes.PreorderedSet
+  Classes.Joinable Classes.Galois Classes.IsNat Psatz.
 
 (** * Parity *)
 
 Inductive parity : Type :=
   | par_even : parity
-  | par_odd : parity
-  | par_top : parity.
+  | par_odd : parity.
 
-Inductive parity_ensemble : parity -> Prop :=
-  | par_ens_all : forall p, parity_ensemble p.
+Inductive gamma_par : parity → ℘ nat :=
+  | gamma_par_even : ∀ n, Nat.Even n → gamma_par par_even n
+  | gamma_par_odd  : ∀ n, Nat.Odd n → gamma_par par_odd n.
+Hint Constructors gamma_par : soundness.
+
+Instance galois_parity_nat : Galois parity nat := gamma_par.
 
 (** ** Operations *)
 
 (** *** Plus *)
 Definition parity_plus (p q : parity) : parity :=
   match p with 
-  | par_top => match q with
-               | _ => par_top
-               end
   | par_even => q
   | par_odd => match q with
-               | par_top => par_top
                | par_even => par_odd
                | par_odd => par_even
                end
   end.
-Hint Unfold parity_plus : soundness.
+Instance parity_plus_op : plus_op parity parity  := parity_plus.
 
-Lemma parity_plus_par_even : forall p,
-  parity_plus p par_even = p.
-Proof. intros. destruct p; reflexivity. Qed.
-
-Corollary parity_plus_par_odd : forall p,
-  parity_plus p par_odd = par_even -> p = par_odd.
+Instance parity_plus_sound : plus_op_sound parity nat.
 Proof.
-  intros; destruct p; try inv H; reflexivity.
-Qed.
-
-Lemma parity_plus_assoc : forall p q r,
-  parity_plus (parity_plus p q) r = parity_plus p (parity_plus q r).
-Proof.
-  destruct p, q, r; try reflexivity.
-Qed.
-
-Lemma parity_plus_comm : forall p q,
-  parity_plus p q = parity_plus q p.
-Proof.
-  destruct p, q; try reflexivity. 
+  intros p q n m Hpn Hqm. destruct p, q. 
+  - cbn. inversion Hpn; subst. constructor. inversion Hqm; subst.
+    unfold plus. unfold nat_plus_op. destruct H.
+    destruct H0. subst. rewrite <- Nat.mul_add_distr_l.
+    econstructor. reflexivity.
+  - cbn. inversion Hpn; subst. inversion Hqm; subst. destruct H, H0; subst.
+    constructor. unfold plus; unfold nat_plus_op.  rewrite plus_assoc.
+    rewrite <- Nat.mul_add_distr_l. econstructor. reflexivity. 
+  - cbn. unfold plus, nat_plus_op. constructor. inversion Hqm; subst. 
+    inversion Hpn; subst. destruct H, H0; subst. rewrite plus_comm. rewrite
+    plus_assoc. rewrite <- Nat.mul_add_distr_l. econstructor. reflexivity.
+  - cbn. constructor. unfold plus, nat_plus_op. inversion Hpn; inversion Hqm;
+    subst. destruct H, H0; subst. rewrite plus_assoc. 
+    replace (Nat.add (Nat.add (Nat.add (Nat.mul 2 x) 1) (Nat.mul 2 x0)) 1) with
+      (S ( S( (Nat.add (Nat.mul 2 x) (Nat.mul 2 x0))))).
+    rewrite <- Nat.mul_add_distr_l. rewrite Nat.Even_succ_succ.
+    econstructor. reflexivity. lia.
 Qed.
 
 Definition parity_mult (p q : parity) : parity :=
   match p with
   | par_even => par_even
   | par_odd => q
-  | par_top => par_top
   end.
-Hint Unfold parity_mult : soundness.
+Instance parity_mult_op : mult_op parity parity := parity_mult.
+
+Instance parity_mult_sound : mult_op_sound parity nat.
+Proof.
+  intros p q n m Hpn Hqm. destruct p, q; cbn; constructor; inversion Hpn;
+  inversion Hqm; destruct H, H0; clear Hpn; clear Hqm; subst; unfold mult,
+  nat_mult_op.
+  - rewrite <- mult_assoc. econstructor; reflexivity.
+  - rewrite <- mult_assoc. econstructor; reflexivity.
+  - rewrite mult_assoc. rewrite (mult_comm (Nat.add (Nat.mul 2 x) 1) 2).
+    rewrite <- mult_assoc. econstructor; reflexivity.
+  - rewrite <- odd_equiv. apply odd_mult; rewrite odd_equiv; econstructor;
+    reflexivity.
+Qed.
 
 (** Equality *)
-Definition parity_eq (p1 p2 : parity) : abstr_bool :=
+Definition parity_eq (p1 p2 : parity) : (abstr_bool+⊤) :=
   match p1, p2 with
-  | par_even, par_odd => ab_false
-  | par_odd, par_even => ab_false
-  | _, _ => ab_top
+  | par_even, par_odd => NotTop ab_false
+  | par_odd, par_even => NotTop ab_false
+  | _, _ => Top
   end.
+Instance parity_eq_op : eq_op parity (abstr_bool+⊤) := parity_eq.
 
-Definition parity_leb (p1 p2 : parity) : abstr_bool :=
-  match p1, p2 with
-  | _, par_top    => ab_true
-  | par_even, par_odd | par_odd, par_even => ab_top
-  | par_even, par_even | par_odd, par_odd => ab_top
-  | par_top, _  => ab_top
-  end.
+Instance parity_eq_sound : eq_op_sound (B:=abstr_bool+⊤) parity nat.
+Proof.
+  intros p q n m Hpn Hqm. destruct p, q; constructor; gamma_destruct; unfold
+  eq, nat_eq_op; rewrite Nat.eqb_neq; unfold not; intro Hnot; subst;
+  apply (Nat.Even_Odd_False m); assumption.
+Qed.
+
+Instance parity_leb_op : leb_op parity (abstr_bool+⊤) := λ _, λ _, Top.
+Instance parity_leb_sound : leb_op_sound (B:=abstr_bool+⊤) parity nat.
+Proof.
+  intros p q n m Hpn Hqm. unfold leb, parity_leb_op, nat_leb_op.
+  constructor.
+Qed.
 
 (* Some lemmas regarding Nat.Even and Nat.Odd that are missing but are included
- * for the deprecated even and odd. We define these lemmas here so we can use the  * newer definitions for when the older version are deleted. *)
-Lemma Even_add : forall n m, Nat.Even n -> Nat.Even m -> Nat.Even (n + m).
+ * for the deprecated even and odd. We define these lemmas here so we can use the  
+ * newer definitions for when the older version are deleted. *)
+(*Lemma Even_add : forall n m, Nat.Even n -> Nat.Even m -> Nat.Even (n + m).
 Proof.
   intros. rewrite <- Nat.even_spec in *. 
   replace true with (Bool.eqb (Nat.even n) (Nat.even m)).
@@ -123,3 +139,38 @@ Qed.
 Hint Resolve Even_add Odd_Odd_add Odd_Even_add Even_Odd_add : soundness.
 Hint Resolve Even_mult_l Even_mult_r Odd_mult : soundness.
 Hint Resolve Nat.Even_Odd_False : soundness. 
+*)
+Inductive parity_le : parity → parity → Prop :=
+  | par_le_even : parity_le par_even par_even
+  | par_le_odd  : parity_le par_odd par_odd. 
+Hint Constructors parity_le : preorders.
+
+Global Instance proset_parity : PreorderedSet parity.
+Proof. proof_preorder parity_le. Defined.
+
+Definition parity_join (p1 p2 : parity) : (parity+⊤) :=
+  match p1, p2 with
+  | par_even, par_even => NotTop par_even
+  | par_odd, par_odd => NotTop par_odd
+  | _, _ => Top
+  end.
+
+Instance parity_joinable : Joinable parity (parity+⊤).
+Proof.
+  split with parity_join. destruct x, y; reflexivity.
+Defined.
+
+Instance join_parity_nat_sound : JoinableSound parity (parity+⊤) nat.
+Proof.
+  intros x y z H. destruct x, y; cbv in *; constructor.
+  - destruct H; inversion H; subst; assumption.
+  - destruct H; inversion H; subst; assumption.
+Qed.
+
+Instance preorder_parity_sound : PreorderSound parity nat.
+Proof.
+  intros x y Hpre n Hgamma. destruct x, y; eauto with soundness; inversion
+  Hpre.
+Qed.
+
+
