Types/State.v
@@ -1,5 +1,136 @@
-Require Import Utf8.
+Require Import Utf8 Classes.Joinable Classes.Monad.
 
 Definition State (S A : Type) := S -> (A * S).
 Definition StateT S M A : Type := S → M (A*S)%type.
 
+Section state_joinable.
+  Context {S A} `{S_joinable : Joinable S S, A_joinable : Joinable A A}.
+
+  Definition state_join (st st' : State S A) : State S A :=
+    fun x => (((fst (st x)) ⊔ (fst (st' x)), 
+              ((snd (st x)) ⊔ (snd (st' x))))).
+  Hint Unfold state_join : soundness.
+
+  Global Instance state_joinable : Joinable (State S A) (State S A).
+  Proof.
+    split with state_join. intros st st'. unfold state_join; simpl.
+    ext. rewrite join_comm. rewrite (join_comm (snd (st x)) _).
+    reflexivity.
+  Defined.
+End state_joinable.
+
+Section State_Monad.
+  Context {S : Type}.
+
+  Definition return_state {A} (a :A) : State S A := 
+    λ st : S, (a, st).
+
+  Definition bind_state {A B} 
+    (m : State S A) (f : A -> State S B) : State S B :=
+    λ st, let (x, st') := (m st) in f x st'.
+
+  Arguments bind_state [A B] m f.
+  Hint Unfold bind_state : soundness.
+
+  Lemma bind_state_id_left : ∀ (A B : Type) (f : A → State S B) (a : A),
+    bind_state (return_state a) f = f a.
+  Proof. simple_solve. Qed.
+
+  Lemma bind_state_id_right : ∀ (A : Type) (m : State S A),
+    bind_state m return_state = m.
+  Proof. simple_solve. Qed.
+
+  Lemma bind_state_assoc : ∀ (A B C : Type) (m : State S A) 
+    (f : A → State S B) (g : B → State S C),
+    bind_state (bind_state m f) g =
+    bind_state m (λ a : A, bind_state (f a) g).
+  Proof. simple_solve. Qed.
+
+  Global Instance monad_state : Monad (State S) :=
+  {
+    bind_id_left := bind_state_id_left;
+    bind_id_right := bind_state_id_right;
+    bind_assoc := bind_state_assoc;
+  }. 
+End State_Monad.
+Hint Unfold bind_state : soundness.
+
+Section Monad_StateT.
+  Context {M} `{M_monad : Monad M}.
+  Context {S : Type}.
+
+  Definition return_stateT {A} (a : A) :=
+    λ st : S, returnM (a, st).
+  Hint Unfold return_stateT : soundness.
+
+  Definition bind_stateT {A B} (m : StateT S M A) 
+    (f : A -> StateT S M B) : StateT S M B :=
+    λ st, m st >>= λ p : (A*S)%type, let (a,st') := p in f a st'.
+  Arguments bind_stateT [A B] m f.
+  Hint Unfold bind_stateT : soundness.
+
+  Lemma bind_stateT_id_left : ∀ (A B : Type) (f : A → StateT S M B) (a : A), 
+    bind_stateT (return_stateT a) f = f a.
+  Proof.
+    autounfold with soundness. intros. ext. 
+    rewrite bind_id_left. reflexivity.
+  Qed.
+  Arguments bind_stateT_id_left [A B] f a.
+
+  Lemma bind_stateT_id_right : ∀ (A : Type) (m : StateT S M A), 
+    bind_stateT m return_stateT = m.
+  Proof.
+    intros. autounfold with soundness. ext.
+    rewrite <- bind_id_right. f_equal. ext. destruct x0.
+    reflexivity.
+  Qed.
+  Arguments bind_stateT_id_right [A] m.
+
+  Lemma bind_stateT_assoc : ∀ (A B C : Type) (m : StateT S M A) 
+    (f : A → StateT S M B) (g : B → StateT S M C),
+    bind_stateT (bind_stateT m f) g =
+    bind_stateT m (λ a : A, bind_stateT (f a) g).
+  Proof.
+    intros. autounfold with soundness. ext.
+    autorewrite with soundness. f_equal. extensionality p.
+    destruct p. reflexivity.
+  Qed.
+  Arguments bind_stateT_assoc [A B C] m f g.
+
+  Global Instance monad_stateT : Monad (StateT S M) :=
+  {
+    bind_id_left := bind_stateT_id_left;
+    bind_id_right := bind_stateT_id_right;
+    bind_assoc := bind_stateT_assoc;
+  }. 
+End Monad_StateT.
+Hint Unfold bind_stateT : soundness.
+
+Section MonadT_StateT.
+  Context {S : Type}.
+
+  Definition lift_stateT {M} `{Monad M} {A} (m : M A) : StateT S M A :=
+    λ st, m >>= λ a, returnM (a, st).
+  Hint Unfold lift_stateT : soundness.
+  
+  Lemma lift_stateT_pure {M} `{Monad M} {A} : ∀ (a : A), 
+    lift_stateT (returnM a) = return_stateT a.
+  Proof.
+    intros. autounfold with soundness. ext.
+    autorewrite with soundness. reflexivity.
+  Qed.
+
+  Lemma lift_stateT_bind {M} `{Monad M} {A B} : ∀ (m : M A) (f : A → M B),
+    lift_stateT (m >>= f) = bind_stateT (lift_stateT m) (f ∘ lift_stateT (A:=B)).
+  Proof.
+    intros. simpl.
+    autounfold with soundness. ext. autorewrite with soundness.
+    f_equal. ext. autorewrite with soundness. reflexivity.
+  Qed.
+
+  Global Instance monadT_stateT : MonadT (StateT S) :=
+  {
+    lift_return := @lift_stateT_pure;
+    lift_bind := @lift_stateT_bind;
+  }. 
+End MonadT_StateT.
