Types/Stores.v
@@ -1,21 +1,47 @@
 Require Export Base.
-Require Import Types.Maps.
+Require Import Types.Maps Language.Statements Classes.Joinable Classes.Galois.
 Require Import Language.Statements.
 
-Definition abstract_store := total_map avalue.
-Definition store := total_map cvalue.
+Definition store (A : Type) := total_map A.
 
-Instance abstract_store_inhabited : Inhabited abstract_store := λ _, VTop.
-Instance concrete_store_inhabited : Inhabited store := λ _, VNat 0.
+Definition store_update {A : Type} (s : store A) (x : string) (v : A) :
+  store A := t_update s x v.
 
-Definition abstract_update (s : abstract_store) (x : string) (v : avalue) :
-  abstract_store := t_update s x v.
+Definition abstract_store := store (avalue_par+⊤).
+Definition concrete_store := store cvalue.
 
-Definition concrete_update (s : store) (x : string) (v : cvalue) :
-  store := t_update s x v.
+Definition gamma_store {A A' B B'} `{Galois A A', Galois B B'} 
+  (st : store A) (st' : store A') : Prop := ∀ x : string, γ (st x) (st' x).
 
-Definition generic_store (A : Type) := total_map A.
+Instance galois_store {A A'} `{Galois A A'} : Galois (store A) (store A') :=
+  gamma_store.
 
-Definition generic_store_update {A : Type} (s : generic_store A) (x : string) (v : A) :
-  generic_store A := t_update s x v.
+Definition store_join {A B} `{Joinable A B} (st1 st2 : store A) : store B :=
+  λ x, (st1 x) ⊔ (st2 x).
+
+Instance store_joinable {A B} `{Joinable A B} : Joinable (store A) (store B).
+Proof.
+  split with store_join. intros x y. unfold store_join. ext. rewrite join_comm.
+  reflexivity.
+Defined.
+
+Instance store_join_sound {A A' B} {JA : Joinable A B} {GA : Galois A A'}
+  {GB :Galois B A'} {JS: JoinableSound A B A'} :
+  JoinableSound (store A) (store B) (store A').
+Proof.
+  intros x y z Hgamma. unfold "⊔"; simpl. unfold store_join. intros s. 
+  apply JS. cbv in Hgamma. destruct Hgamma.
+  - left; apply H.
+  - right. apply H.
+Qed.
+
+Lemma store_update_sound {A A'} `{Galois A A'} :
+  ∀ (st : store A) (st' : store A') x p n,
+  γ st st' →
+  γ p n →
+  γ (store_update st x p) (store_update st' x n).
+Proof.
+  unfold store_update, t_update. intros. unfold γ, galois_store, gamma_store. 
+  intros x'. destruct (beq_string x x'); eauto with soundness.
+Qed.
 
