Base.v
@@ -74,29 +74,6 @@ Ltac simple_solve := autounfold with soundness; intros;
  * and unbounded, we set an upperbound here to avoid infinite loops *)
 Global Set Typeclasses Depth 10.
 
-Class Inhabited (S : Type) := inhabitent : S.
-Arguments inhabitent _ {_}.
-
-Class SubType (sub : Type) (super : Type) : Type := {
-  inject : sub → super;
-  project : super → option sub
-}.
-
-Instance subtype_l : ∀ {A B}, SubType A (A + B) := {
-  inject := inl;
-  project := λ s, match s with | inl x => Some x | _ => None end
-}.
-
-Instance subtype_self : ∀ {A}, SubType A A := {
-  inject := id;
-  project := λ x, Some x
-}.
-
-Instance subtype_r : ∀ {A B C} `{SubType A B}, SubType A (C + B) := {
-  inject := inject ∘ inr;
-  project := λ s, match s with | inr x => project x | _ => None end
-}.
-
 Class top_op (A:Type) : Type := top : A.
 Notation "⊤" := top (at level 40).
 
@@ -113,6 +90,78 @@ Inductive botlift (A:Type) : Type :=
 Arguments Bot {A}.
 Arguments NotBot {A}.
 Notation "t +⊥" := (botlift t) (at level 39).
+
+Section top_bot_coercions.
+  Context {A : Type}.
+
+  Definition A_to_top (a : A) : (A+⊤) := NotTop a.
+  Coercion A_to_top : A >-> toplift.
+
+  Definition A_to_bot (a : A) : (A+⊥) := NotBot a.
+  Coercion A_to_bot : A >-> botlift.
+End top_bot_coercions.
+
+Class SubType (sub : Type) (super : Type) : Type := {
+  inject : sub → super;
+  project : super → option sub
+}.
+
+Instance subtype_l : ∀ {A B}, SubType A (A + B) := {
+  inject := inl;
+  project := λ s, match s with | inl x => Some x | _ => None end
+}.
+
+Instance subtype_r : ∀ {A B}, SubType B (A+B) := {
+  inject := inr;
+  project := λ s, match s with | inr x => Some x | _ => None end
+}.
+
+Instance subtype_trans_r : ∀ {A B C} `{SubType A B}, SubType A (C + B) := {
+  inject := inject ∘ inr;
+  project := λ s, match s with | inr x => project x | _ => None end
+}.
+
+Instance subtype_trans_l {A B C} `{S : SubType A B} : SubType A (B + C).
+Proof. destruct S as [inject project]. split.
+  - exact (λ a, inl (inject a)).
+  - exact (λ bc, match bc with
+                 | inr _ => None
+                 | inl b => project b
+                 end).
+Defined.
+
+Instance subtype_top_r : ∀ A, SubType A (A+⊤) := {
+  inject := NotTop;
+  project := λ a, match a with
+                  | Top => None
+                  | NotTop x => Some x
+                  end;
+}.
+
+Instance subtype_bot_r : ∀ A, SubType A (A+⊥) := {
+  inject := NotBot;
+  project := λ a, match a with
+                  | Bot => None
+                  | NotBot x => Some x
+                  end;
+}.
+
+Instance subtype_top_l {A B} `{SubType A B} : 
+  SubType (A+⊤) (B+⊤).
+Proof. destruct H as [inject project]. split.
+  exact (λ a : (A+⊤), match a with
+                      | Top => Top
+                      | NotTop x => NotTop( inject x)
+                      end).
+  exact (λ b : (B+⊤), match b with
+                      | Top => None
+                      | NotTop x => match (project x) with
+                                    | Some x' => Some (NotTop x')
+                                    | None => None
+                                    end
+                      end).
+Defined.
+
 
 Notation "℘ A" := (A → Prop) (at level 0, only parsing).
 Definition union {U : Type} (A B : U → Prop) : U → Prop :=
