Classes/Monad/MonadState.v
@@ -1,4 +1,4 @@
-Require Export Coq.Strings.String.
+Require Export Base Coq.Strings.String.
 Require Import Classes.Monad.
 
 Class MonadState (S : Type) (M : Type -> Type) `{M_monad : Monad M} :=
