Classes/SoundMonad.v
@@ -5,17 +5,3 @@ Require Import Classes.Monad.
 Require Import Classes.Monad.MonadFail.
 Require Import Instances.Galois.
 
-Section sound_monad.
-  Context (M M' : Type → Type) `{M_fail : MonadFail M, M'_fail : MonadFail M'}.
-  Context {M_preorder : ∀ T', PreorderedSet T' → PreorderedSet (M' T')}.
-  Context {M_galois : ∀ T T' {HT : PreorderedSet T'}, Galois T T' → Galois (M T) (M' T')}.
-
-  Class SoundMonad : Type :=
-  {
-    return_sound : ∀ (A A' : Type) `{Galois A A'},
-      γ (returnM (M:=M') (A:=A')) (returnM (M:=M) (A:=A));
-    bind_sound : ∀ (A A' B B' : Type) `{Galois A A', Galois B B'},
-      γ (bindM (M:=M') (A:=A') (B:=B')) (bindM (M:=M) (A:=A) (B:=B));
-  }.
-End sound_monad.
-Hint Resolve return_sound bind_sound : soundness.
